theories/util/fancy_lists.v
@@ -62,6 +62,27 @@ Fixpoint lget {A} (Xl: list A) : pidx Xl → A :=
   match Xl with [] => absurd |
     X :: Xl' => λ i, match i with PO => X | PS j => lget Xl' j end end.
 
+(** * Equal Length Witness *)
+
+Fixpoint eq_len_wit {A B} (Xl: list A) (Yl: list B) : Set :=
+  match Xl, Yl with [], [] => () |
+    _ :: Xl', _ :: Yl' => eq_len_wit Xl' Yl' | _, _ => ∅ end.
+
+Lemma of_eq_len_wit `{Xl: _ A} `{Yl: _ B} :
+  eq_len_wit Xl Yl → length Xl = length Yl.
+Proof.
+  move: Xl Yl. fix FIX 1. case=> [|??]; case=>//= ???. f_equal. by apply FIX.
+Qed.
+Lemma to_eq_len_wit `{Xl: _ A} `{Yl: _ B} :
+  length Xl = length Yl → eq_len_wit Xl Yl.
+Proof.
+  move: Xl Yl. fix FIX 1. case=> [|??]; case=>//= ??[=?]. by apply FIX.
+Qed.
+
+Fixpoint symm_eq_len_wit `{Xl: _ A} `{Yl: _ B} :
+  eq_len_wit Xl Yl → eq_len_wit Yl Xl := match Xl, Yl with [], [] => λ _, () |
+    _ :: Xl', _ :: Yl' => λ e, symm_eq_len_wit (e: _ Xl' Yl') | _, _ => absurd end.
+
 (** * Heterogeneous List *)
 
 Inductive hlist {A} (F: A → Type) : list A → Type :=
@@ -209,9 +230,15 @@ Lemma papply_app `{F: A → _} {B Xl Yl}
 Proof. move: fl. elim Xl; [done|]=>/= ?? IH [??]. by rewrite IH. Qed.
 
 Fixpoint plist_map `{F: A → _} {Xl Yl} :
-  plist2 (λ A B, F A → F B) Xl Yl → plist F Xl → plist F Yl :=
+  plist2 (λ X Y, F X → F Y) Xl Yl → plist F Xl → plist F Yl :=
   match Xl, Yl with [], [] => λ _, id
   | _ :: _, _ :: _ => λ '(f -:: fl') '(x -:: xl'), f x -:: plist_map fl' xl'
+  | _, _ => absurd end.
+
+Fixpoint plist_map_with `{F: A → _} {G} {Xl Yl} (h: ∀X Y, G X Y → F X → F Y) :
+  plist2 G Xl Yl → plist F Xl → plist F Yl :=
+  match Xl, Yl with [], [] => λ _, id
+  | _ :: _, _ :: _ => λ '(f -:: fl') '(x -:: xl'), h _ _ f x -:: plist_map_with h fl' xl'
   | _, _ => absurd end.
 
 Fixpoint hzip_with {A} {F G H: A → Type} {Xl} (f: ∀X, F X → G X → H X)
@@ -219,13 +246,33 @@ Fixpoint hzip_with {A} {F G H: A → Type} {Xl} (f: ∀X, F X → G X → H X)
   match xl, yl with +[], _ => +[] |
     x +:: xl', y -:: yl' => f _ x y +:: hzip_with f xl' yl' end.
 
+Fixpoint plist2_eq_len_wit `{F: A → _} {Xl Yl} : plist2 F Xl Yl → eq_len_wit Xl Yl :=
+  match Xl, Yl with [], [] => λ _, () |
+    _ :: _, _ :: _ => λ '(_ -:: xl'), plist2_eq_len_wit xl' | _, _ => absurd end.
+
+Lemma plist2_eq_len `{F: A → _} {Xl Yl} : plist2 F Xl Yl → length Xl = length Yl.
+Proof. by move=> /plist2_eq_len_wit/of_eq_len_wit ?. Qed.
+
+
 (** * Uniform plist *)
 
 Definition plistc {B} (A: Type) (Xl: list B) : Type := plist (const A) Xl.
 
-Fixpoint plistc_to_vec {B A} {Xl: _ B} : plistc A Xl → vec A (length Xl) :=
-  match Xl with [] => const [#] | _ :: _ => λ '(x -:: xl), x ::: plistc_to_vec xl end.
+Fixpoint plistc_to_vec {B A} {Xl: _ B} (xl: plistc A Xl) : vec A (length Xl) :=
+  match Xl, xl with [], _ => [#] | _ :: _, x -:: xl' => x ::: plistc_to_vec xl' end.
 Coercion plistc_to_vec: plistc >-> vec.
+
+Fixpoint plistc_renew {A} `{Xl: _ B} `{Yl: _ C}
+  : eq_len_wit Xl Yl → plistc A Xl → plistc A Yl :=
+  match Xl, Yl with [], [] => λ _ _, -[] |
+    _ :: Xl', _ :: Yl' => λ e '(x -:: xl'), x -:: plistc_renew (e: _ Xl' Yl') xl' |
+    _, _ => absurd end.
+
+Lemma plistc_renew_eq {A} `{Xl: _ B} `{Yl: _ C} (xl: _ A _) (e: _ Xl Yl) :
+  (plistc_renew e xl: list _) = xl.
+Proof.
+  move: Xl Yl e xl. fix FIX 1. case=> [|??]; case=>//= ???[??]/=. f_equal. apply FIX.
+Qed.
 
 (** * Vector *)
 
@@ -298,13 +345,12 @@ Proof.
 Qed.
 
 Fixpoint psum_map `{F: A → _} {Xl Yl} :
-  plist2 (λ A B, F A → F B) Xl Yl → psum F Xl → psum F Yl :=
+  plist2 (λ X Y, F X → F Y) Xl Yl → psum F Xl → psum F Yl :=
   match Xl, Yl with [], [] => λ _, absurd
   | _ :: _, _ :: _ => λ '(f -:: fl'), sum_map f (psum_map fl')
   | _, _ => absurd end.
 
-Lemma psum_map_pinj `{F: A → _} {Xl Yl} (fl: plist2 (λ A B, F A → F B) Xl Yl)
-  (i: p2idx Xl Yl) (x: F (lget Xl (p2fin_l i))) :
+Lemma psum_map_pinj `{F: A → _} {Xl Yl} (fl: _ Xl Yl) i (x: F _) :
   psum_map fl (pinj (p2fin_l i) x) = pinj (p2fin_r i) (p2get fl i x).
 Proof.
   move: Xl Yl fl i x. fix FIX 1. move=> [|??] [|??] /= fl; case=> [|?];
@@ -359,11 +405,6 @@ Proof. move=> All. move: i. elim All; [done|]=> > ???. by case. Qed.
 Lemma HForallTwo_get `{F: A → _} {G Xl} (Φ: ∀X, F X → G X → Prop) (xl yl: _ Xl) i :
   HForallTwo Φ xl yl → Φ _ (hget xl i) (hget yl i).
 Proof. move=> All. move: i. elim All; [done|]=> > ???. by case. Qed.
-
-Lemma HForall2_1_eq_len `{F: A → _} {G H Xl Yl}
-  (Φ: ∀X Y, F X → G Y → H X Y → Prop) (xl: _ Xl) (yl: _ Yl) zl :
-  HForall2_1 Φ xl yl zl → length Xl = length Yl.
-Proof. by elim; [done|]=>/= > ??->. Qed.
 
 Lemma HForallTwo_forall `{!Inhabited Y} `{F: A → _} {G Xl}
   (Φ: ∀X, Y → F X → G X → Prop) (xl yl: _ Xl) :
